platform/cito/Label2Word.v
@@ -1,0 +1,40 @@
+Set Implicit Arguments.
+
+Require Import IL Memory Word.
+Require Import GLabel ConvertLabel.
+
+Section stn.
+
+  Variable Domain : glabel -> Prop.
+
+  Variable stn : settings.
+
+  Definition stn_injective :=
+    forall lbl1 lbl2 p, 
+      Domain lbl1 -> 
+      Domain lbl2 -> 
+      Labels stn lbl1 = Some p -> 
+      Labels stn lbl2 = Some p -> 
+      lbl1 = lbl2.
+
+  Definition labels (lbl : glabel) : option W := Labels stn lbl.
+  
+  Definition is_label_map_to_word lbl p :=
+    match labels lbl with
+      | Some p' => 
+        if weq p p' then
+          true
+        else
+          false
+      | None => false
+    end.
+
+  Definition is_label_map_to_word' A p (x : glabel * A) := is_label_map_to_word (fst x) p.
+
+  Definition find_by_word A m (p : W) : option A :=
+    match List.find (is_label_map_to_word' p) m with
+      | Some (_, a) => Some a
+      | None => None
+    end.
+
+End stn.
